Consider two bodies of [[mass|masses]] $m_{1}$ and $m_{2}$ moving in $\mathbb{R}^{3}$, for a total of $n=6$ [[degrees of freedom]]. Each position vector is $\mathbf{r}_{i}=(x_{i},y_{i},z_{i})$ for $i=1,2$. The [[kinetic energy]] is
$$T=\frac{1}{2}m_{1} \dot{\mathbf{r}}_{1}^{2}+ \frac{1}{2}m_{2}\dot{\mathbf{r}}_{2}^{2}$$
The [[potential energy]] is dependent on the distance between the bodies, $V\equiv V(\mathbf{r}_{1}-\mathbf{r}_{2})=V(\mathbf{r})$, where we defined $\mathbf{r}\equiv \mathbf{r}_{1}-\mathbf{r}_{2}$ for the sake of brevity. Like in most $N$-body systems, we can use the [[center of mass]] frame to simplify our treatment. Call $M\equiv m_{1}+m_{2}$ the total mass. The center of mass is located by
$$\mathbf{R}=\frac{m_{1}\mathbf{r}_{1}+m_{2}\mathbf{r}_{2}}{M}$$
We can retroactively get the positions of the two bodies from the center of mass as
$$\mathbf{r}_{1}=\mathbf{R}+ \frac{m_{2}\mathbf{r}}{M},\qquad \mathbf{r}_{2}=\mathbf{R}- \frac{m_{1}\mathbf{r}}{M}$$
With these new coordinates, we can rewrite the expression of kinetic energy in this frame:
$$\begin{align}
T&=\frac{1}{2}m_{1}\left( \dot{\mathbf{R}}^{2}+ \cancel{ \frac{2m_{2}}{M}\dot{\mathbf{R}}\cdot\dot{\mathbf{r}} }+ \frac{m_{2}^{2}}{M}\dot{\mathbf{r}}^{2} \right)+ \frac{1}{2}m_{2}\left( \dot{\mathbf{R}}^{2}- \cancel{ \frac{2m_{1}}{M}\dot{\mathbf{R}}\cdot \dot{\mathbf{r}} }+ \frac{m_{1}^{2}}{M}\dot{\mathbf{r}}^{2} \right) \\
&=\frac{1}{2}M \dot{\mathbf{R}}^{2}+ \frac{1}{2} \frac{m_{1}m_{2}^{2}+m_{2}m_{1}^{2}}{M^{2}}\dot{\mathbf{r}}^{2}
\end{align}$$
We now defined the reduced mass $\mu\equiv m_{1}m_{2}/M$, with which we can comfortably write
$$T=\frac{1}{2}M \dot{\mathbf{R}}^{2}+ \frac{1}{2}\mu \dot{\mathbf{r}}^{2}$$
The kinetic energy has gone from the sums if kinetic energy of the bodies to the sums of kinetic energy of the "center of mass" and of another terms that evidently takes up "everything else". With the kinetic energy known, we are ready to write the [[Lagrangian]] of this system:
$$L=\frac{1}{2}M \dot{\mathbf{R}}^{2}+ \frac{1}{2}\mu \dot{\mathbf{r}}^{2}- V(\mathbf{r})$$
for some potential energy $V$. Note that this does not depend on *where* the center of mass is, as there is no mention of $\mathbf{R}$ (only its derivative $\dot{\mathbf{R}}$).

We can interpret this equation as the sum of a free particle of mass $M$ and a particle of mass $\mu$ subject to a potential $V(\mathbf{r})$. In this light, we'll split the Lagrangian in two. Specifically, the latter part is
$$L(\mathbf{r},\dot{\mathbf{r}})=\frac{1}{2}\mu \lvert \dot{\mathbf{r}} \rvert ^{2}-V(\lvert \mathbf{r} \rvert )$$
As with all Lagrangians, our priority should be sniff out [[Constant of motion|constants of motion]], as each and every one we find makes our problem easier. This Lagrangian of $\mathbf{r}$, for instance, is invariant to [[Rotation|rotations]] (in $SO(3)$). Invoking [[NÃ¶ther's theorem]], this means that the [[angular momentum]] $\mathbf{A}$[^1] is a constant of motion (all three components actually, so $A_{x}$, $A_{y}$ and $A_{z}$). Let's analyze what this invariance implies. The momentum is $\mathbf{A}=\mu \mathbf{r}\times \dot{\mathbf{r}}$. If it's constant over $\mathbf{r}(t)$, then $\mu \mathbf{r}(t)\times \dot{\mathbf{r}}(t)=\mathbf{A}_\text{const}$, but for a [[vector product]] to give an angle-independent constant we must have both $\mathbf{r}(t)$ and $\dot{\mathbf{r}}(t)$ lying [[Orthogonality|orthogonal]] to $\mathbf{A}_\text{const}$. In other words, both $\mathbf{r}(t)$ and $\dot{\mathbf{r}}(t)$ (and by extension the whole motion) lie on a plane perpendicular to $\mathbf{A}_\text{const}$.

This bit of geometry gives us the information that we need to simplify our coordinates. We'll then pick a [[frame of reference]] in which $(A_\text{const})_{x}=(A_\text{const})_{y}=0$[^2]. In this frame, we can pick the canonical [[basis]] $\{ \mathbf{e}_{x} ,\mathbf{e}_{y}\}$ and express $\mathbf{r}$ and $\dot{\mathbf{r}}$ as a [[linear combination]] of these:
$$\mathbf{r}=x\mathbf{e}_{x}+y\mathbf{e}_{y},\qquad \dot{\mathbf{r}}=\dot{x}\mathbf{e}_{x}+\dot{y}\mathbf{e}_{y}$$
In here, the Lagrangian becomes
$$L=\frac{1}{2}\mu(\dot{x}^{2}+\dot{y}^{2})- V(\sqrt{ x^{2}+y^{2} })$$
Since we're on a plane, we might as well move to [[polar coordinates]]. The appropriate [[coordinate transformation]] is
$$x=r\cos \theta,\qquad y=r\sin \theta$$
for which
$$L=\frac{1}{2}\mu(\dot{r}^{2}+r^{2}\dot{\theta}^{2})-V(r)$$
You might be wondering why the switch: the answer is that our "$\mu$" particle is moving in a straight line. Of course: there's no angular momentum, it can't be rotating! So our angular coordinate must be *[[Lagrangian|cyclical]]* and, as such, its [[Conjugate momenta|conjugate momentum]] is another constant of motion:
$$p_{\theta}=\frac{ \partial L }{ \partial \theta } =mr^{2}\dot{\theta}\equiv l=\text{constant}$$
As usual, this leads to an easy first order [[Ordinary differential equation|ODE]]:
$$\dot{ \theta}=\frac{l}{mr^{2}}$$
We can look for an effective Lagrangian
$$\begin{align}
L_\text{eff}&=L-\left.{\dot{\theta}l}\right|_{\dot{ \theta}=l/mr^{2}} \\
&=\frac{1}{2}m \dot{ r}^{2}+ \frac{m}{2}r^{2} \frac{l^{2}}{(mr^{2})^{2}}-V(r)- \frac{l^{2}}{mr^{2}} \\
&=\frac{1}{2}m \dot{r}^{2}- V(r)- \frac{l^{2}}{2mr^{2}} \\
&=\frac{1}{2}m \dot{r}^{2}-V_\text{eff}(r)
\end{align}$$
where
$$V_\text{eff}(r)=V(r)+\frac{l^{2}}{2mr^{2}}$$
Solving the [[Lagrange equation]] yields $r(t)$, which we can put into $\dot{\theta}$ to get
$$\dot{\theta}(t)=\frac{l}{mr(t)^{2}}$$
which we can solve to find $\theta(t)$. More importantly, $\theta(t)$ is invertible so we can find $t(\theta)$. Since $r(\theta(t)))$ is a composite function, we can use the [[chain rule]]:
$$\dot{r}(t)=\frac{d}{d\theta}r(\theta(t))\dot{\theta }(t)=\frac{dr}{d\theta} \frac{l}{mr^{2}}=- \frac{l}{m} \left.{\frac{d}{d\theta}\left( \frac{1}{r} \right)}\right|_{\theta=\theta(t)}$$
and
$$\ddot{r}(t)=- \frac{l}{m} \frac{d^{2}}{d\theta ^{2}}\left( \frac{1}{r} \right)\dot{\theta}=- \frac{l^{2}}{m^{2}r^{2}} \left.{\frac{d^{2}}{d\theta ^{2}}\left( \frac{1}{r} \right)}\right|_{\theta=\theta(t)}$$
Specifically when $\ddot{r}(t(\theta))$ we have
$$\ddot{r}(t(\theta))=- \frac{l^{2}}{m^{2}r^{2}} \frac{d^{2}}{d\theta ^{2}}\left( \frac{1}{r} \right)$$
### Keplerian potential
This is about as far as we get without knowing the specifics of the system. Everything up until now is perfectly general, provided the system matches our specifications. We now need some form of potential to keep going: we'll use a Keplerian potential to analyze gravitationally bound (or unbound) systems like [[Pianeta|planets]] around a [[stella|star]]. We start with a qualitative analysis of the one dimensional analog of potential
$$V(r)=- \frac{k}{r}$$
for some constant $k>0\in \mathbb{R}$. Our effective potential then is
$$V_\text{eff}(r)=- \frac{k}{r}+ \frac{l^{2}}{2mr^{2}}$$
There's a few cases of interest here that are already well known from classical mechanics depending on the total energy $E$ of the system.

![[Diagram Gravitational system]]

$E_{1}$ is the circular orbit case. In that case
$$\dot{\theta}(t)=\frac{l}{mr(t)^{2}}=\frac{l}{mr_{0}^{2}}\quad\to \quad \theta(t)=\frac{l}{mr_{0}^{2}}t+\theta_{0}$$
where $r_{0}$ is the constant orbit distance and $\theta_{0}$ is the starting angle.

$E_{2}$ is the elliptic orbit case. Here, the solution is similar to $E_{1}$ but $r(t)$ is no longer constant.

$E_{3}$ and $E_{4}$ are known as **collision events**. This is because the orbits may end up passing through the source point of the potential (the "star" so to speak) and collide with it. It doesn't necessarily need to happen however, and they may also described open orbits that only do a single pass near the star and then leave forever. $E_{3}$ is the specific case where the orbit is exactly parabolic.

Now, to actually quantitatively solve for the motion itself, we need to tackle the Lagrange equation. The actual equation to solve is
$$\frac{d}{dt} \frac{ \partial L_\text{eff} }{ \partial \dot{r} } =m \ddot{r}\quad\to \quad \ddot{r}=- \frac{k}{mr^{2}}+ \frac{l^{2}}{m^{2}r^{3}}$$
and
$$\frac{ \partial L_\text{eff} }{ \partial r } =- \frac{k}{r^{2}}+ \frac{l^{2}}{m^{3}}$$
The condition that $r(\theta)$ needs to satisfy then is
$$- \frac{l^{2}}{m^{2}r^{2}} \frac{d^{2}}{d\theta ^{2}}\left( \frac{1}{r} \right)=- \frac{k}{mr^{2}}+ \frac{l^{2}}{m^{2}r^{3}}$$
which when rearranged is
$$\frac{d^{2}}{d\theta ^{2}}\left( \frac{1}{r} \right)= \frac{km}{l^{2}}- \frac{1}{r}$$
Since it's all reliant on $1/r$, we'll define $1/r(\theta)\equiv u(\theta)$ and $km/l^{2}=1/\eta$. With these symbols, our ODE simplifies to
$$u''+u=\frac{1}{\eta}$$
This leads to the solution
$$u(\theta)=\frac{1}{\eta}+ \frac{e}{\eta}\cos(\theta-\theta_{0})$$
for some value $e$. If we put $1/r(\theta)$ back in we finally get our orbit:
$$\boxed{r(\theta)=\frac{\eta}{1+e\cos(\theta-\theta_{0})}}$$
This is the general expression for a [[conic]] (the geometric shape), where $e$ is the eccentricity. When $0\leq e< 1$ we get an ellipse ($E_{1}$ and $E_{2}$), when $e=1$ we get a parabola ($E_{3}$) and for $e>1$ we get a hyperbole ($E_{4}$).


[^1]: Unfortunately, both common letters for angular momentum, $L$ and $M$, are taken here so we'll use the less orthodox $\mathbf{A}$ here (it stands for "angular").

[^2]: Mathematically, this is a [[level set]] of codimension $2$.
